theories/CScoping.v
@@ -2,8 +2,6 @@
 
   Stating that all variables are in a given cscope, and in a given mode.
 
-  TODO: Using cscoping is going to conflict with cscoping...
-
 **)
 
 From Coq Require Import Utf8 List.
@@ -14,92 +12,44 @@ Import ListNotations.
 
 Set Default Goal Selector "!".
 
-(* Inductive cscoping (Γ : cscope) : cterm → cmode → Prop :=
+Inductive ccscoping (Γ : cscope) : cterm → cmode → Prop :=
 
 | cscope_var :
     ∀ x m,
       nth_error Γ x = Some m →
-      scoping Γ (var x) m
+      ccscoping Γ (cvar x) m
 
 | scpoe_sort :
     ∀ m i,
-      scoping Γ (Sort m i) mKind
+      ccscoping Γ (cSort m i) cType
 
 | cscope_pi :
     ∀ i j mx m A B,
-      scoping Γ A mKind →
-      scoping (mx :: Γ) B mKind →
-      scoping Γ (Pi i j m mx A B) mKind
+      ccscoping Γ A cType →
+      ccscoping (mx :: Γ) B cType →
+      ccscoping Γ (cPi i j m mx A B) cType
 
 | cscope_lam :
     ∀ mx m A B t,
-      scoping Γ A mKind →
-      scoping (mx :: Γ) B mKind →
-      scoping (mx :: Γ) t m →
-      scoping Γ (lam mx A B t) m
+      ccscoping Γ A cType →
+      ccscoping (mx :: Γ) B cType →
+      ccscoping (mx :: Γ) t m →
+      ccscoping Γ (clam mx A B t) m
 
 | cscope_app :
     ∀ mx m t u,
-      scoping Γ t m →
-      scoping Γ u mx →
-      scoping Γ (app t u) m
-
-| cscope_erased :
-    ∀ A,
-      scoping Γ A mKind →
-      scoping Γ (Erased A) mKind
-
-| cscope_erase :
-    ∀ t,
-      scoping Γ t mType →
-      scoping Γ (erase t) mGhost
-
-| cscope_reveal :
-    ∀ m t P p,
-      In m [ mProp ; mGhost ] →
-      scoping Γ t mGhost →
-      scoping Γ P mKind →
-      scoping Γ p m →
-      scoping Γ (reveal t P p) m
-
-| cscope_revealP :
-    ∀ t p,
-      scoping Γ t mGhost →
-      scoping Γ p mKind →
-      scoping Γ (revealP t p) mKind
-
-| cscope_gheq :
-    ∀ A u v,
-      scoping Γ A mKind →
-      scoping Γ u mGhost →
-      scoping Γ v mGhost →
-      scoping Γ (gheq A u v) mKind
-
-| cscope_ghrefl :
-    ∀ A u,
-      scoping Γ A mKind →
-      scoping Γ u mGhost →
-      scoping Γ (ghrefl A u) mProp
-
-| cscope_ghcast :
-    ∀ m A u v e P t,
-      m ≠ mKind →
-      scoping Γ A mKind →
-      scoping Γ u mGhost →
-      scoping Γ v mGhost →
-      scoping Γ e mProp →
-      scoping Γ P mKind →
-      scoping Γ t m →
-      scoping Γ (ghcast e P t) m
+      ccscoping Γ t m →
+      ccscoping Γ u mx →
+      ccscoping Γ (capp t u) m
 
 | cscope_bot :
-    scoping Γ bot mKind
+    ccscoping Γ cbot cType
 
 | cscope_bot_elim :
     ∀ m A p,
-      scoping Γ A mKind →
-      scoping Γ p mProp →
-      scoping Γ (bot_elim m A p) m
+      ccscoping Γ A cType →
+      ccscoping Γ p cProp →
+      ccscoping Γ (cbot_elim m A p) m
 .
 
-Notation cscoping Γ := (scoping (sc Γ)). *)
+Notation ccxscoping Γ := (ccscoping (sc Γ)).
